theories/sim/local.v
@@ -1,16 +1,171 @@
 From Paco Require Export paco.
+From iris.algebra Require Import cmra gmap csum agree excl.
 
-From stbor.sim Require Export invariant local_base.
+From stbor.lang Require Import defs.
 
 Set Default Proof Using "Type".
 
-Definition sim_body := sim_local_body wsat vrel_expr.
-Definition sim_fun := sim_local_fun wsat vrel_expr.
-Definition sim_funs := sim_local_funs wsat vrel_expr.
+Section local.
+Context {A: ucmraT}.
+Variable (wsat: A → state → state → Prop).
+Variable (vrel: A → expr → expr → Prop).
+Variable (fns_src fns_tgt: fn_env).
+
+(* TODO: encode what it means for the context to not contain our private tags! *)
+(* TODO: how do we know we're at the top of the stack? *)
+Inductive _sim_local_body
+  (sim_local_body : A → expr → state → expr → state → Prop)
+  (r: A) : expr → state → expr → state → Prop :=
+(* If src is stuck, then anything is related *)
+| sim_local_body_stuck e_src σ_src e_tgt σ_tgt
+    (STUCK: stuck e_src (mkConfig fns_src σ_src))
+    : _sim_local_body sim_local_body r e_src σ_src e_tgt σ_tgt
+(* If tgt makes 1 step, src can make some step *)
+| sim_local_body_step e_src σ_src e_tgt σ_tgt
+    (STEP: ∀ r_f e_tgt' cfg_tgt'
+      (* for any frame r_f that is compatible with our resource r and has world satisfaction *)
+      (VALID: ✓ (r_f ⋅ r)) (WSAT: wsat (r_f ⋅ r) σ_src σ_tgt)
+      (* if tgt can locally make 1 step *)
+      (STEPT: (e_tgt, (mkConfig fns_tgt σ_tgt)) ~t~> (e_tgt', cfg_tgt')),
+      (* then we locally can makes some step and pick a new resource r' *)
+      ∃ e_src' cfg_src' r',
+        (e_src, (mkConfig fns_src σ_src)) ~t~>* (e_src', cfg_src') ∧
+        ✓ (r_f ⋅ r') ∧ wsat (r_f ⋅ r') cfg_src'.(cst) cfg_tgt'.(cst) ∧
+        sim_local_body r' e_src' cfg_src'.(cst) e_tgt' cfg_tgt'.(cst))
+    : _sim_local_body sim_local_body r e_src σ_src e_tgt σ_tgt
+(* If tgt prepares to make a call to [name], src should be able to make the same
+  call. Here we do not want to step into the call of [name], but to step over it. *)
+| sim_local_body_step_over_call K_src K_tgt fid e_src e_tgt el_tgt σ_src σ_tgt
+    (CALLTGT: e_tgt = fill K_tgt (Call #[ScFnPtr fid] el_tgt))
+    (STEPOVER: ∀ r_f
+        (* for any frame r_f that is compatible with our resource r and has world satisfaction *)
+        (VALID: ✓ (r_f ⋅ r))
+        (WSAT : wsat (r_f ⋅ r) σ_src σ_tgt)
+        (* tgt is ready to make a call of [name] *)
+        (VTGT : Forall (λ ei, is_Some (to_value ei)) el_tgt),
+        (* then src is also ready to make a call of [name] *)
+        ∃ el_src cfg_src rc rv,
+        (e_src, (mkConfig fns_src σ_src)) ~t~>*
+          (fill K_src (Call #[ScFnPtr fid] el_src), cfg_src) ∧
+        Forall (λ ei, is_Some (to_value ei)) el_src ∧
+        (* and we can pick a resource [rv] for the arguments *)
+        ✓ (r_f ⋅ (rc ⋅ rv)) ∧ wsat (r_f ⋅ (rc ⋅ rv)) cfg_src.(cst) σ_tgt ∧
+        (* [rv] justifies the arguments *)
+        Forall2 (vrel rv) el_src el_tgt ∧
+        (* and after the call our context can continue *)
+        (∀ r_f' r' v_src v_tgt cfg_src' cfg_tgt'
+          (* For any new resource r' and frame r_f' that are compatible with
+             our local resource r and has world satisfaction *)
+          (VALID': ✓ (r_f' ⋅ (rc ⋅ r')))
+          (WSAT' : wsat (r_f ⋅ (rc ⋅ r')) cfg_src'.(cst) cfg_tgt'.(cst))
+          (* and the returned values are related w.r.t. (r ⋅ r' ⋅ r_f) *)
+          (VRET  : vrel r' (Val v_src) (Val v_tgt)),
+          sim_local_body (rc ⋅ r')
+                      (fill K_src (Val v_src)) cfg_src'.(cst)
+                      (fill K_tgt (Val v_tgt)) cfg_tgt'.(cst)))
+    : _sim_local_body sim_local_body r e_src σ_src e_tgt σ_tgt
+(* If tgt prepares to end, src also prepares to end *)
+| sim_local_body_end_call v_src σ_src v_tgt σ_tgt e_src e_tgt
+    (ESRC: e_src = EndCall (Val v_src))
+    (ETGT: e_tgt = EndCall (Val v_tgt))
+    (END: ∀ r_f cfg_tgt'
+        (VALID: ✓ (r_f ⋅ r))
+        (WSAT : wsat (r_f ⋅ r) σ_src σ_tgt)
+        (* if tgt can end call *)
+        (ETGT: (EndCall (Val v_tgt), (mkConfig fns_tgt σ_tgt)) ~t~> cfg_tgt'),
+        (* then src can also end call *)
+        ∃ cfg_src' r',
+        (EndCall (Val v_src), (mkConfig fns_src σ_tgt)) ~t~> cfg_src' ∧
+        (* and re-establish wsat *)
+        ✓ (r_f ⋅ r') ∧ wsat (r_f ⋅ r') cfg_src'.2.(cst) cfg_tgt'.2.(cst) ∧
+        (* and the returned values are related *)
+        vrel r' (Val v_src) (Val v_tgt))
+    : _sim_local_body sim_local_body r e_src σ_src e_tgt σ_tgt
+.
+
+Lemma sim_local_body_mono : monotone5 _sim_local_body.
+Proof.
+  intros r es σs et σt R R' SIM LE; inversion SIM; subst.
+  - by eapply sim_local_body_stuck; eauto.
+  - eapply sim_local_body_step. naive_solver.
+  - eapply sim_local_body_step_over_call; eauto. naive_solver.
+  - by eapply sim_local_body_end_call; eauto.
+Qed.
+
+Definition sim_local_body := paco5 _sim_local_body bot5.
+
+Lemma sim_local_body_resource_mono r1 r2
+  (SAT_DOWNWARD: ∀ r1 r2, r1 ≼ r2 → wsat r2 <2= wsat r1) :
+  r1 ≼ r2 → sim_local_body r1 <4= sim_local_body r2.
+Proof.
+  revert r1 r2. pcofix CIH. intros r1 r2 LE es σs et σt SIM.
+  pfold. punfold SIM; [|apply sim_local_body_mono].
+  inversion SIM; subst.
+  - by eapply sim_local_body_stuck.
+  - eapply sim_local_body_step.
+    intros r_f et' ct' VL2 WS2 STEPT.
+    have VL1: ✓ (r_f ⋅ r1).
+    { eapply cmra_valid_included; [exact VL2|by apply cmra_mono_l]. }
+    have WS1: wsat (r_f ⋅ r1) σs σt.
+    { eapply SAT_DOWNWARD; [by apply cmra_mono_l|exact WS2]. }
+    destruct (STEP _ _ _ VL1 WS1 STEPT) as (es' & cs' & r' & STEPS' & VL' & WS' & SIM').
+    exists es', cs', r'. do 3 (split; [done|]).
+    right. eapply CIH; eauto. by inversion SIM'.
+  - eapply sim_local_body_step_over_call; eauto.
+    intros r_f VL2 WS2 FAT.
+    have VL1: ✓ (r_f ⋅ r1).
+    { eapply cmra_valid_included; [exact VL2|by apply cmra_mono_l]. }
+    have WS1: wsat (r_f ⋅ r1) σs σt.
+    { eapply SAT_DOWNWARD; [by apply cmra_mono_l|exact WS2]. }
+    destruct (STEPOVER _ VL1 WS1 FAT)
+      as (es' & cs & rc & rv & STEPS & FAS & VL & WS & VREL & HK).
+    exists es', cs, rc, rv. do 5 (split; [done|]).
+    intros r_f' r' vs vt cs' ct' VL' WS' VREL'.
+    specialize (HK _ _ _ _ _ _ VL' WS' VREL').
+    right. eapply CIH; [eauto|by inversion HK].
+  - eapply sim_local_body_end_call; [eauto..|].
+    intros r_f ct' VL2 WS2 STEPT.
+    have VL1: ✓ (r_f ⋅ r1).
+    { eapply cmra_valid_included; [exact VL2|by apply cmra_mono_l]. }
+    have WS1: wsat (r_f ⋅ r1) σs σt.
+    { eapply SAT_DOWNWARD; [by apply cmra_mono_l|exact WS2]. }
+    naive_solver.
+Qed.
+
+(* Simulating functions: assuming the calls have been initialized. *)
+Definition sim_local_fun (fn_src fn_tgt : function) : Prop :=
+  ∀ r e_src e_tgt el_src el_tgt σ_src σ_tgt
+    (VALS: Forall (λ ei, is_Some (to_value ei)) el_src)
+    (VALT: Forall (λ ei, is_Some (to_value ei)) el_tgt)
+    (VALEQ: Forall2 (vrel r) el_src el_tgt)
+    (EQS: match fn_src with
+          | FunV xl e => subst_l xl el_src e = Some e_src
+          end)
+    (EQT: match fn_tgt with
+          | FunV xl e => subst_l xl el_tgt e = Some e_tgt
+          end),
+    sim_local_body r (InitCall e_src) σ_src (InitCall e_tgt) σ_tgt.
+
+Definition sim_local_funs : Prop :=
+  ∀ name fn_src, fns_src !! name = Some fn_src → ∃ fn_tgt,
+    fns_tgt !! name = Some fn_tgt ∧ sim_local_fun fn_src fn_tgt.
+
+End local.
+
+Hint Resolve sim_local_body_mono : paco.
 
 Definition init_state := (mkState ∅ ∅ [] O O).
 
+Section program.
+Context {A: ucmraT}.
+Variable (wsat: A → state → state → Prop).
+Variable (vrel: A → expr → expr → Prop).
+
 (* Program simulation: All functions are related, and so is initialization. *)
-Definition sim_prog (prog_src prog_tgt: fn_env) : Prop :=
-  sim_funs prog_src prog_tgt ∧
-  sim_body prog_src prog_tgt ε (Call #["main"] []) init_state (Call #["main"] []) init_state.
+Record sim_prog (prog_src prog_tgt: fn_env) := {
+  sim_prog_env: sim_local_funs wsat vrel prog_src prog_tgt;
+  sim_prog_main:
+    sim_local_body wsat vrel prog_src prog_tgt ε
+                   (Call #["main"] []) init_state (Call #["main"] []) init_state;
+}.
+End program.
